SharedInterpreter.v
@@ -1,0 +1,50 @@
+Require Import Language.
+Require Import Monad.
+
+Fixpoint shared_aexp (S V : Type)
+  (extraction : nat -> V)
+  (plus_op mult_op : V -> V -> V)
+  (e : aexp) :=
+  match e with 
+  | ANum n => returnM (extraction n)
+  | AVar x =>
+      st << get ;
+      returnM (st x)
+  | APlus e1 e2 =>
+      v1 << (shared_aexp S V extraction plus_op mult_op e1) ;
+      v2 << (shared_aexp S V extraction plus_op mult_op e2) ;
+      returnM (plus_op v1 v2)
+  | AMult e1 e2 =>
+      v1 << (shared_aexp S V extraction plus_op mult_op e1) ;
+      v2 << (shared_aexp S V extraction plus_op mult_op e2) ;
+      returnM (mult_op v1 v2)
+  end.
+  
+(*Fixpoint shared_bexp (S BV NV : Type) 
+  (extract_b : bool -> BV)
+  (extract_n : nat -> NV)
+  (equals_op : NV -> NV -> BV)
+  (le_op : NV -> NV -> BV)
+  (neg_op : BV -> BV)
+  (and_op : BV -> BV -> BV)
+  (e : bexp) :
+  State S BV :=
+  match e with
+  | BTrue => returnM (extraction true)
+  | BFalse => returnM (extraction false)
+  | BEq e1 e2 =>
+      v1 << (shared_aexp S NV extract_n equals_op le_op neg_op and_op e1) ;
+      v2 << (shared_aexp S NV extract_n equals_op le_op neg_op and_op e2) ;
+      returnM (equals_op v1 v2)
+  | BLe e1 e2 =>
+      v1 << (shared_aexp S BN NV extraction equals_op le_op neg_op and_op e1) ;
+      v2 << (shared_aexp S BN NV extraction equals_op le_op neg_op and_op e2) ;
+      returnM (le_op v1 v2)
+  | BNot b1 =>
+      v1 << (shared_bexp S BN NV extraction equals_op le_op neg_op and_op b1) ;
+      returnM (neg_op v1)
+  | BAnd b1 b2 =>
+      v1 << (shared_bexp S BN NV extraction equals_op le_op neg_op and_op b1) ;
+      v2 << (shared_bexp S BN NV extraction equals_op le_op neg_op and_op b2) ;
+      returnM (and_op v1 v2)
+  end.*)
